Tweak monadic presentation of dataLang programs

compiler/backend/semantics/data_monadScript.sml
@@ -1,72 +1,105 @@
 (*
   Define a monad to make dataLang ASTs nicer to work with
 *)
-open preamble dataLangTheory dataSemTheory ml_monadBaseTheory;
+open preamble dataLangTheory dataSemTheory;
 
 val _ = new_theory"data_monad";
 
-val s = ``s:('c,'ffi) dataSem$state``
-val f = ``(f: (('c,'ffi) dataSem$state, unit, (v,v) result) M)``
-val g = ``(g: (('c,'ffi) dataSem$state, unit, (v,v) result) M)``
+Type M = ``:('c,'ffi) dataSem$state -> (v, v) result option # ('c,'ffi) dataSem$state``
 
-Definition Corr_def:
-  Corr ast ^f <=>
-    !^s. evaluate (ast, s) =
-           case f s of
-           | (Success (), s1) => (NONE, s1)
-           | (Failure res, s1) => (SOME res, s1)
-End
+val s = ``s:('c,'ffi) dataSem$state``
+val f = ``f: ('c,'ffi) M``
+val g = ``g: ('c,'ffi) M``
 
 Definition skip_def[simp]:
-  (skip : (('c,'ffi) dataSem$state, unit, (v,v) result) M) s =
-    (Success (), s)
+  (skip : ('c,'ffi) M) s =
+    (NONE, s)
+End
+
+Definition fail_def[simp]:
+  (fail : ('c,'ffi) M) s =
+    (SOME (Rerr(Rabort Rtype_error)), s)
 End
 
 Definition bind_def:
   bind ^f ^g s =
     case f s of
-    | (Failure res, s1) => (Failure res, s1)
-    | (Success _, s1) => g s1
+    | (SOME res, s1) => (SOME res, s1)
+    | (NONE, s1) => g s1
+End
+
+Definition if_var_def:
+  if_var n ^f ^g s =
+    case lookup n s.locals of
+    | NONE => fail s
+    | SOME v => if isBool T v then f s else
+                if isBool F v then g s else fail s
 End
 
 Definition return_def[simp]:
   return n s =
     case lookup n s.locals of
-    | NONE => (Failure (Rerr(Rabort Rtype_error)), s)
-    | SOME v => (Failure (Rval v), s with locals := LN)
+    | NONE => fail s
+    | SOME v => (SOME (Rval v), s with locals := LN)
 End
 
 Definition tailcall_def:
   tailcall dest args ^s =
     case get_vars args s.locals of
-    | NONE => (Failure (Rerr(Rabort Rtype_error)), s)
+    | NONE => fail s
     | SOME vs =>
       case find_code dest vs s.code of
-      | NONE => (Failure (Rerr(Rabort Rtype_error)), s)
+      | NONE => fail s
       | SOME (args,prog) =>
           if s.clock = 0 then
-            (Failure (Rerr(Rabort Rtimeout_error)),
+            (SOME (Rerr(Rabort Rtimeout_error)),
              s with <| stack := [] ; locals := LN |>)
           else
-            case evaluate (prog, call_env args (dec_clock s)) of
-            | (NONE, s1) => (Failure (Rerr(Rabort Rtype_error)), s1)
-            | (SOME r, s1) => (Failure r, s1)
+            let (res,s) = evaluate (prog, call_env args (dec_clock s)) in
+              if res = NONE then fail s else (res,s)
 End
+
+Definition assign_def:
+  assign dest (op, args, names_opt) s =
+    if op_requires_names op /\ IS_NONE names_opt then fail s else
+      case cut_state_opt names_opt s of
+      | NONE => fail s
+      | SOME s =>
+        case get_vars args s.locals of
+        | NONE => fail s
+        | SOME xs =>
+          case do_app op xs s of
+          | Rerr e => (SOME (Rerr e), s with <| stack := []; locals := LN |>)
+          | Rval (v,s) => (NONE, set_var dest v s))
+End
+
+Overload ":=" = ``assign``
+val _ = set_fixity ":=" (Infixl 480);
 
 Definition to_shallow_def:
   to_shallow Skip = skip /\
+  to_shallow (Assign n op vars cutset) = assign n (op, vars, cutset) /\
   to_shallow (Seq p1 p2) = bind (to_shallow p1) (to_shallow p2) /\
   to_shallow (Return n) = return n /\
-  to_shallow (Call NONE dest args NONE) = tailcall dest args
+  to_shallow (Call NONE dest args NONE) = tailcall dest args /\
+  to_shallow (Call NONE dest args (SOME x)) = fail /\
+  to_shallow (If n p1 p2) = if_var n (to_shallow p1) (to_shallow p2) /\
+  to_shallow c = ARB c "not yet done..."
 End
 
-Theorem Corr_thm:
-  !ast. Corr ast (to_shallow ast)
+Theorem to_shallow_thm:
+  !ast ^s. evaluate (ast, s) = to_shallow ast s
 Proof
-  Induct \\ fs [to_shallow_def,Corr_def,evaluate_def]
+  Induct \\ fs [to_shallow_def,evaluate_def]
   \\ rpt gen_tac
   THEN1 cheat
-  THEN1 cheat
+  THEN1
+   (rename [`Call ret dest args handler`]
+    \\ Cases_on `ret` THEN1
+     (reverse (Cases_on `handler`) \\ fs [to_shallow_def]
+      \\ fs [tailcall_def]
+      \\ rpt (TOP_CASE_TAC \\ fs [call_env_def,fromList_def]))
+    \\ cheat)
   THEN1 cheat
   THEN1 cheat
   THEN1 cheat
@@ -78,11 +111,23 @@ Proof
   THEN1 cheat
 QED
 
-(* Overload monad_bind[local] = ``st_ex_bind`` *)
-(* Overload monad_ignore_bind[local] = ``\x y. st_ex_bind x (\z. y)`` *)
-Overload monad_unitbind[local] = ``\x y. bind x y``
+Overload monad_unitbind[local] = ``bind``
 Overload return[local] = ``return``
 
 val _ = monadsyntax.temp_add_monadsyntax()
+
+val challenge_program =
+  ``Seq (Assign 2 (TagLenEq 0 0) [0] NONE)
+        (If 2 (Return 1)
+              (Seq (Assign 5 (Const 0) [] NONE)
+              (Seq (Assign 3 El [0; 5] NONE)
+              (Seq (Assign 5 (Const 1) [] NONE)
+              (Seq (Assign 6 El [0; 5] NONE)
+              (Seq (Assign 4 (Cons 0) [5; 1] NONE)
+                   (Call NONE (SOME 500) [6; 4] NONE)))))))``
+
+val to_shallow_thm =
+  ``to_shallow ^challenge_program``
+  |> REWRITE_CONV [to_shallow_def]
 
 val _ = export_theory();
